{-# OPTIONS --without-K --exact-split --safe #-}

module N-order where

open import Universes public
open import MLTT public
open Arithmetics renaming(_+_ to _+Ì‡_)

_â‰¤_ _â‰¥_ : â„• -> â„• -> ğ’°â‚€ Ì‡

infix 10 _â‰¤_
infix 10 _â‰¥_

{-
-- wtf 
_â‰¤_ = â„•-iteration (â„• -> ğ’°â‚€ Ì‡) (Î» y -> ğŸ™) (Î» f -> â„•-recursion (ğ’°â‚€ Ì‡) ğŸ˜ (Î» y P -> f y))
-}

zero â‰¤ y = ğŸ™
succ x â‰¤ zero = ğŸ˜
succ x â‰¤ succ y = x â‰¤ y

x â‰¥ y = y â‰¤ x 

-- Strict inequalities
_<_ _>_ : â„• -> â„• -> ğ’°â‚€ Ì‡
infix 10 _<_
infix 10 _>_

x < zero = ğŸ˜
zero < succ y = ğŸ™
succ x < succ y = x < y

x > y = y < x

-- Proving the rest of the Peano axioms for â„•
familyâ„•â†’ğ’° : â„• -> ğ’°â‚€ Ì‡
familyâ„•â†’ğ’° 0 = ğŸ˜
familyâ„•â†’ğ’° (succ n) = â„•

positivesNotZero : (x : â„•) -> (succ x) â‰¢ 0
positivesNotZero x p = transport familyâ„•â†’ğ’° p x

-- Lifting succs
succUp : (x y : â„•) -> x â‰¡ y -> (succ x) â‰¡ (succ y)
succUp zero zero eq = refl (succ 0)
succUp (succ x) (succ .x) (refl .(succ x)) = refl (succ (succ x))

succLess : {x y : â„•} -> succ x â‰¡ succ y -> x â‰¡ y
succLess {x} {.x} (refl .(succ x)) = refl x

-- Note that the fith axiom is just â„•-induction

â„•-hasDecidableEquality : hasDecidableEq â„•
â„•-hasDecidableEquality zero zero = inl (refl 0)
â„•-hasDecidableEquality zero (succ n1) = inr (â‰¢-sym (positivesNotZero n1))
â„•-hasDecidableEquality (succ n0) zero = inr (positivesNotZero n0)
â„•-hasDecidableEquality (succ n0) (succ n1) = f (â„•-hasDecidableEquality n0 n1)
    where
        f : decidable (n0 â‰¡ n1) -> decidable (succ n0 â‰¡ succ n1)
        f (inl p) = inl (ap succ p)
        f (inr fâ‚š) = inr (Î» (s : succ n0 â‰¡ succ n1) -> fâ‚š (succLess s))

-- prove antisymmetry of strict ordering
<asym : (x y : â„•) -> x < y -> Â¬(y < x)
<asym zero (succ y) l = id
<asym (succ x) (succ y) l = <asym x y l

â‰¤refl : {x : â„•} -> x â‰¤ x -> x â‰¤ x
â‰¤refl l = l

â‰¤asym : (x y : â„•) -> x â‰¤ y -> (x â‰¡ y -> ğŸ˜) -> (y â‰¤ x -> ğŸ˜) 
â‰¤asym zero zero * ne = Î» _ -> ne (refl 0)
â‰¤asym zero (succ y) * ne = id
â‰¤asym (succ x) (succ y) l ne = â‰¤asym x y l (Î» eq -> ne (succUp x y eq))

â‰¤trans : (x y z : â„•) -> x â‰¤ y -> y â‰¤ z -> x â‰¤ z
â‰¤trans zero zero zero l k = *
â‰¤trans zero zero (succ z) l k = *
â‰¤trans zero (succ y) (succ z) l k = *
â‰¤trans (succ x) (succ y) (succ z) l k = â‰¤trans x y z l k

-- Prove the following: x â‰¤ y if and only if Î£ z ê‰ â„• , x + z â‰¡ y.

{-
â‰¤ToÎ£ : (x y : â„•) -> x â‰¤ y -> Î£ z :- â„• , (x +Ì‡ z â‰¡ y)
â‰¤ToÎ£ zero zero leq = (0 , refl 0)
â‰¤ToÎ£ zero (succ y) leq = {!   !}
â‰¤ToÎ£ (succ x) (succ y) leq = {!   !}
-}